theories/Compositional_Structures/Sequential_Composition_Ref.thy
@@ -5,11 +5,12 @@ theory Sequential_Composition_Ref
 begin
 
 
-definition sequential_composition_mon :: "'a Electoral_Module_Ref \<Rightarrow> 'a Electoral_Module_Ref \<Rightarrow>
+
+definition sequential_composition_ref :: "'a Electoral_Module_Ref \<Rightarrow> 'a Electoral_Module_Ref \<Rightarrow>
         'a Electoral_Module_Ref" where
-"sequential_composition_mon m n A p = do {
+"sequential_composition_ref m n A p = do {
       new_A <- (defer_monadic m) A p;
-      new_p <- limit_profile_l A p;  
+      new_p <- limit_profile_l new_A p;  
                         
       electmA  <- (elect_monadic m) A p;
       electnA' <- (elect_monadic n) new_A new_p;
@@ -19,11 +20,28 @@ definition sequential_composition_mon :: "'a Electoral_Module_Ref \<Rightarrow> 
 
       defernA'  <- (defer_monadic n) new_A new_p;
 
-      RETURN (electmA \<union> electnA',rejectmA \<union> rejectnA',defernA')}"
+      RETURN (electmA \<union> electnA',rejectmA \<union> rejectnA',defernA')
+}"
 
 
-
-
+definition sequential_composition_ref_test :: "'a Electoral_Module_Ref \<Rightarrow> 'a Electoral_Module_Ref \<Rightarrow>
+        'a Electoral_Module_Ref" where
+"sequential_composition_ref_test m n A p = do {
+      mresulte <- m A p;
+      mresultr <- m A p;
+      
+      m'result <- m A p;
+      
+      let newA = (defer_r (m'result));
+      new_p <- limit_profile_l newA p;  
+      
+      nresulte <- n newA new_p;
+      nresultr <- n newA new_p;
+      nresultd <- n newA new_p;
+      
+      RETURN (elect_r mresulte \<union> elect_r nresulte, reject_r mresultr \<union> reject_r nresultr
+      , defer_r nresultd)
+}"
 
 locale seqcomp_impl =
   fixes m_ref :: "nat Electoral_Module_Ref"
@@ -45,39 +63,99 @@ begin
 
   lemma this_loc: "seqcomp_impl m_ref m_impl n_ref n_impl" by unfold_locales
 
-interpretation m_sel: set_select_imp m_ref m_impl 
-  using m_impl by (unfold_locales, simp)
-
-interpretation n_sel:  set_select_imp n_ref n_impl 
-  using n_impl by (unfold_locales, simp)
-
-(*sepref_register "m_ref" :: "nat Electoral_Module_Ref"
-sepref_register "n_ref" :: "nat Electoral_Module_Ref"
-
+sepref_register "m_ref" :: "nat Electoral_Module_Ref"
 declare m_impl [sepref_fr_rules]
-declare n_impl [sepref_fr_rules]*)
 
-sepref_register "(elect_monadic m_ref)"
+sepref_register "n_ref" :: "nat Electoral_Module_Ref"
+declare n_impl [sepref_fr_rules]
 
-declare local.m_sel.elect_sep.refine [sepref_fr_rules]
+schematic_goal sequence_impl: "(uncurry ?seq,  uncurry (sequential_composition_ref_test m_ref n_ref))
+  \<in> alts_set_impl_assn\<^sup>k *\<^sub>a (profile_impl_assn)\<^sup>k \<rightarrow>\<^sub>a (result_impl_assn)"
+  unfolding sequential_composition_ref_test_def defer_monadic_def elect_monadic_def reject_monadic_def
+  apply sepref_dbg_keep
+  done
 
-schematic_goal seqcomp_imp:
-  "(uncurry ?c, (uncurry (sequential_composition_mon m_ref n_ref))) 
-    \<in> alts_set_impl_assn\<^sup>k *\<^sub>a (profile_impl_assn)\<^sup>k \<rightarrow>\<^sub>a (result_impl_assn)"
-  unfolding sequential_composition_mon_def  defer_monadic_def reject_monadic_def
-  by sepref
-
-concrete_definition (in -) sequential_composition_sep uses seqcomp_impl.seqcomp_imp
+concrete_definition (in -) sequential_composition_sep uses seqcomp_impl.sequence_impl
   prepare_code_thms (in -) sequential_composition_sep_def
 lemmas seqt_imp_refine = sequential_composition_sep.refine[OF this_loc]
 
-
-
-
-thm sequential_composition_sep_def
-
-
 end 
+
+locale sequence_refine = seqcomp_impl +
+  fixes m :: "nat Electoral_Module"  and
+  n :: "nat Electoral_Module"
+assumes module_m: "electoral_module m"
+  and module_n: "electoral_module n"
+assumes m_ref_correct: "(uncurry m_ref, uncurry (RETURN oo m)) \<in> 
+  ([\<lambda> (A, pl). finite_profile A
+            pl]\<^sub>f (\<langle>nat_rel\<rangle>set_rel \<times>\<^sub>r profile_rel)
+   \<rightarrow> \<langle>\<langle>nat_rel\<rangle>set_rel \<times>\<^sub>r \<langle>nat_rel\<rangle>set_rel \<times>\<^sub>r \<langle>nat_rel\<rangle>set_rel\<rangle>nres_rel)" and
+n_ref_correct: "(uncurry n_ref, uncurry (RETURN oo n)) \<in> 
+  ([\<lambda> (A, pl). finite_profile A
+            pl]\<^sub>f (\<langle>nat_rel\<rangle>set_rel \<times>\<^sub>r profile_rel)
+   \<rightarrow> \<langle>\<langle>nat_rel\<rangle>set_rel \<times>\<^sub>r \<langle>nat_rel\<rangle>set_rel \<times>\<^sub>r \<langle>nat_rel\<rangle>set_rel\<rangle>nres_rel)"
+
+begin
+
+lemma seq_comp_correct:
+  shows "(uncurry (sequential_composition_ref m_ref n_ref),
+  uncurry (RETURN oo (sequential_composition m n)))
+  \<in>   ([\<lambda> (A, pl). finite_profile A
+            pl]\<^sub>f (\<langle>nat_rel\<rangle>set_rel \<times>\<^sub>r profile_rel)
+   \<rightarrow> \<langle>\<langle>nat_rel\<rangle>set_rel \<times>\<^sub>r \<langle>nat_rel\<rangle>set_rel \<times>\<^sub>r \<langle>nat_rel\<rangle>set_rel\<rangle>nres_rel)"
+  unfolding sequential_composition_ref_def
+proof (intro frefI nres_relI,clarsimp simp del: limit_profile.simps, rename_tac A pl pr,
+    unfold SPEC_eq_is_RETURN(2)[symmetric], refine_vcg)
+  fix A :: "nat set"
+  fix pl :: "nat Profile_List"
+  fix pr :: "nat Profile"
+  assume prel: "(pl, pr) \<in> profile_rel"
+  assume fina: "finite A"
+  assume profa: "profile A pr"
+  note mrc = m_ref_correct[THEN frefD, THEN nres_relD]
+  note drc = defer_monadic_correct[THEN frefD, THEN nres_relD]
+  from fina prel profa have "defer_monadic m_ref A pl \<le> SPEC (\<lambda> dset. dset = defer m A pr)"
+    unfolding SPEC_eq_is_RETURN(2) using m_ref_correct drc[where emref2 = m_ref and em2 = m and x1 = "(A, pl)"
+        and y1 = "(A, pr)"]
+    by auto
+  let ?new_A = "defer m A pr"
+  let ?new_p = "limit_profile ?new_A pr"
+  have fin_def: "finite ?new_A"
+    using def_presv_fin_prof fina profa module_m
+    by metis
+  have prof_def_lim:
+    "profile (defer m A pr) (limit_profile (defer m A pr) pr)"
+    using def_presv_fin_prof fina profa module_m
+    by metis
+  from fina prel profa have "limit_profile_l ?new_A pl \<le> 
+    \<Down> profile_rel (SPEC (\<lambda> lim. lim = limit_profile (defer m A pr) pr))"
+    unfolding SPEC_eq_is_RETURN(2) using limitp_correct[THEN frefD, THEN nres_relD, where  x1 = 
+        "(A, pl)"
+        and y1 = "(A, pr)"]
+    unfolding comp_apply 
+  from prel fina profa show "defer_monadic m_ref A pl
+       \<le> SPEC (\<lambda>new_A.
+                   limit_profile_l new_A pl \<bind>
+                   (\<lambda>new_p.
+                       elect_monadic m_ref A pl \<bind>
+                       (\<lambda>electmA.
+                           elect_monadic n_ref new_A new_p \<bind>
+                           (\<lambda>electnA'.
+                               reject_monadic m_ref A pl \<bind>
+                               (\<lambda>rejectmA.
+                                   reject_monadic n_ref new_A new_p \<bind>
+                                   (\<lambda>rejectnA'.
+                                       defer_monadic n_ref new_A new_p \<bind>
+                                       (\<lambda>defernA'.
+                                           SPEC
+                                            (\<lambda>x. x = (electmA \<union> electnA', rejectmA \<union> rejectnA',
+  defernA'))))))))
+                   \<le> SPEC (\<lambda>x. x = (let new_A = defer m A pr; new_p = limit_profile new_A pr
+                                     in (elect m A pr \<union> elect n new_A new_p,
+                                         reject m A pr \<union> reject n new_A new_p, defer n new_A new_p))))"
+ 
+
+end
 
 
 abbreviation sequence_sep
